src/linear/impl/LinkedList.dfy
@@ -29,16 +29,18 @@ trait LinkedListIterator extends ListIterator {
     requires forall it | it in Parent().Repr() :: allocated(it)
     ensures Parent().Valid()
     ensures Valid()
-    ensures old(Index()) < Index()
     ensures old(Parent()) == Parent()
     ensures old(Parent().Model()) == Parent().Model()
+
+    ensures forall x {:trigger x in Parent().Repr(), x in old(Parent().Repr())} | x in Parent().Repr() - old(Parent().Repr()) :: fresh(x)
+    ensures fresh(Parent().Repr()-old(Parent().Repr()))
+    ensures forall x | x in Parent().Repr() :: allocated(x)
+
     ensures Parent().Iterators() == old(Parent().Iterators())
     ensures x == Parent().Model()[old(Index())]
     ensures Index() == 1 + old(Index())
     ensures forall it | it in Parent().Iterators() && old(it.Valid()) ::
       it.Valid() && (it != this ==> it.Index() == old(it.Index()))
-    ensures forall x | x in Parent().Repr() - old(Parent().Repr()) :: fresh(x)
-    ensures forall x | x in Parent().Repr() :: allocated(x)
 
   function method Peek(): int
     reads this, Parent(), Parent().Repr()
@@ -53,10 +55,17 @@ trait LinkedListIterator extends ListIterator {
     requires Parent().Valid()
     requires allocated(Parent())
     requires forall it | it in Parent().Iterators() :: allocated(it)
+
     ensures fresh(it)
     ensures Valid()
     ensures it.Valid()
     ensures Parent().Valid()
+    ensures Parent().Model() == old(Parent().Model())
+
+    ensures forall x {:trigger x in Parent().Repr(), x in old(Parent().Repr())} | x in Parent().Repr() - old(Parent().Repr()) :: fresh(x)
+    ensures fresh(Parent().Repr()-old(Parent().Repr()))
+    ensures forall x | x in Parent().Repr() :: allocated(x)
+
     ensures it in Parent().Iterators()
     ensures Parent().Iterators() == {it} + old(Parent().Iterators())
     ensures Parent() == old(Parent())
@@ -65,53 +74,9 @@ trait LinkedListIterator extends ListIterator {
     ensures it.Valid()
     ensures forall it | it in old(Parent().Iterators()) && old(it.Valid()) ::
       it.Valid() && it.Index() == old(it.Index())
-    ensures Parent().Model() == old(Parent().Model())
-    ensures forall x | x in Parent().Repr() - old(Parent().Repr()) :: fresh(x)
-    ensures forall x | x in Parent().Repr() :: allocated(x)
 }
 
 trait LinkedList extends List {
-  /*
-  function ReprDepth(): nat
-    ensures ReprDepth() > 0
-
-  function ReprFamily(n: nat): set<object>
-    decreases n
-    requires n <= ReprDepth()
-    ensures n > 0 ==> ReprFamily(n) >= ReprFamily(n-1)
-    reads this, if n == 0 then {} else ReprFamily(n-1)
-
-  function Repr(): set<object>
-    reads this, ReprFamily(ReprDepth()-1)
-  {
-    ReprFamily(ReprDepth())
-  }
-
-  lemma UselessLemma()
-    ensures Repr() == ReprFamily(ReprDepth());
-
-  predicate Valid()
-    reads this, Repr()
-
-  function Model(): seq<int>
-    reads this, Repr()
-    requires Valid()
-
-  function method Empty(): bool
-    reads this, Repr()
-    requires Valid()
-    ensures Empty() <==> Model() == []
-
-  function method Size(): nat
-    reads this, Repr()
-    requires Valid()
-    ensures Size() == |Model()|
-
-  function Iterators(): set<LinkedListIterator>
-    reads this, Repr()
-    requires Valid()
-    ensures forall it | it in Iterators() :: it in Repr() && it.Parent() == this
-  */
 
   method Begin() returns (it: ListIterator)
     modifies this, Repr()
@@ -119,6 +84,11 @@ trait LinkedList extends List {
     requires forall x | x in Repr()::allocated(x)
     ensures Valid()
     ensures Model() == old(Model())
+
+    ensures forall x {:trigger x in Repr(), x in old(Repr())}| x in Repr() - old(Repr()) :: fresh(x)
+    ensures fresh(Repr()-old(Repr()))
+    ensures forall x | x in Repr() :: allocated(x)
+
     ensures fresh(it)
     ensures Iterators() == {it} + old(Iterators())
     ensures it.Valid()
@@ -126,8 +96,6 @@ trait LinkedList extends List {
     ensures it.Parent() == this
     ensures forall it | it in old(Iterators()) && old(it.Valid()) ::
       it.Valid() && it.Index() == old(it.Index())
-    ensures forall x | x in Repr() - old(Repr()) :: fresh(x)
-    ensures forall x | x in Repr() :: allocated(x)
 
   function method Front(): int
     reads this, Repr()
@@ -143,7 +111,8 @@ trait LinkedList extends List {
     ensures Valid()
     ensures Model() == [x] + old(Model())
 
-    ensures forall x | x in Repr() - old(Repr()) :: fresh(x)
+    ensures forall x {:trigger x in Repr(), x in old(Repr())} | x in Repr() - old(Repr()) :: fresh(x)
+    ensures fresh(Repr()-old(Repr()))
     ensures forall x | x in Repr() :: allocated(x)
 
     ensures Iterators() == old(Iterators())
@@ -158,7 +127,8 @@ trait LinkedList extends List {
     ensures Valid()
     ensures [x] + Model() == old(Model())
 
-    ensures forall x | x in Repr() - old(Repr()) :: fresh(x)
+    ensures forall x {:trigger x in Repr(), x in old(Repr())} | x in Repr() - old(Repr()) :: fresh(x)
+    ensures fresh(Repr()-old(Repr()))
     ensures forall x | x in Repr() :: allocated(x)
 
     ensures Iterators() == old(Iterators())
@@ -179,7 +149,8 @@ trait LinkedList extends List {
     ensures Valid()
     ensures Model() == old(Model()) + [x]
 
-    ensures forall x | x in Repr() - old(Repr()) :: fresh(x)
+    ensures forall x {:trigger x in Repr(), x in old(Repr())} | x in Repr() - old(Repr()) :: fresh(x)
+    ensures fresh(Repr()-old(Repr()))
     ensures forall x | x in Repr() :: allocated(x)
 
     ensures Iterators() == old(Iterators())
@@ -198,7 +169,8 @@ trait LinkedList extends List {
     ensures Valid()
     ensures Model() + [x] == old(Model())
 
-    ensures forall x | x in Repr() - old(Repr()) :: fresh(x)
+    ensures forall x {:trigger x in Repr(), x in old(Repr())} | x in Repr() - old(Repr()) :: fresh(x)
+    ensures fresh(Repr()-old(Repr()))
     ensures forall x | x in Repr() :: allocated(x)
 
     ensures Iterators() == old(Iterators())
@@ -224,6 +196,11 @@ trait LinkedList extends List {
     requires forall x | x in Repr() :: allocated(x)
     ensures Valid()
     ensures Model() == Seq.Insert(x, old(Model()), old(mid.Index()))
+
+    ensures forall x {:trigger x in Repr(), x in old(Repr())} | x in Repr() - old(Repr()) :: fresh(x)
+    ensures fresh(Repr()-old(Repr()))
+    ensures forall x | x in Repr() :: allocated(x)
+
     ensures Iterators() == old(Iterators())
     ensures forall it | it in Iterators() && old(it.Valid()) :: it.Valid()
     ensures forall it | it in Iterators() && old(it.Valid()) ::
@@ -231,301 +208,30 @@ trait LinkedList extends List {
         it.Index() == old(it.Index())
       else
         it.Index() == old(it.Index()) + 1
-    ensures forall x | x in Repr() - old(Repr()) :: fresh(x)
+
+  // Deletion of mid
+  method Erase(mid: ListIterator) returns (next:ListIterator)
+    modifies this, Repr()
+    requires Valid()
+    requires mid.Valid()
+    requires mid.Parent() == this
+    requires mid.HasNext()
+    requires mid in Iterators()
+    requires forall x | x in Repr() :: allocated(x)
+    ensures Valid()
+    ensures Model() == Seq.Remove(old(Model()), old(mid.Index()))
+
+    ensures forall x {:trigger x in Repr(), x in old(Repr())} | x in Repr() - old(Repr()) :: fresh(x)
+    ensures fresh(Repr()-old(Repr()))
     ensures forall x | x in Repr() :: allocated(x)
-}
 
-method FillArray(l: List, v: array<int>)
-  modifies l, l.Repr(), v
-  requires {v} !! {l} + l.Repr()
-  requires l.Valid()
-  requires v.Length == |l.Model()|
-  requires forall x | x in l.Repr() :: allocated(x)
-  ensures l.Valid()
-  ensures l.Model() == old(l.Model())
-  ensures v[..] == l.Model()
-  ensures forall x | x in l.Repr() - old(l.Repr()) :: fresh(x)
-  ensures forall x | x in l.Repr() :: allocated(x)
-  ensures {v} !! {l} + l.Repr()
-{
-
-  ghost var rep := l.Repr();
-
-  var it := l.Begin();
-
-  assert v in l.Repr() - old(l.Repr()) ==> fresh(v);
-
-  var i := 0;
-  while it.HasNext()
-    decreases |l.Model()| - it.Index()
-    invariant l.Valid()
-    invariant l.Model() == old(l.Model())
-    invariant it.Parent() == l
-    invariant it.Valid()
-    invariant {it} !! {l}
-    invariant {v} !! {l} + l.Repr()
-    invariant {v} !! {it}
-    invariant it.Index() == i
-    invariant i <= |l.Model()|
-    invariant v[..i] == l.Model()[..i]
-    invariant forall x | x in l.Repr() - old(l.Repr()) :: fresh(x)
-    invariant forall x | x in l.Repr() :: allocated(x)
-  {
-    ghost var rep2 := l.Repr();
-
-    var x := it.Next();
-
-    reprProgression(rep,rep2,l.Repr());
-    assert v in l.Repr() - old(l.Repr()) ==> fresh(v);
-
-    v[i] := x;
-    i := i + 1;
-  }
-}
-
-
-
-method IteratorExample1(l: List)
-  modifies l, l.Repr()
-  requires l.Valid()
-  requires l.Model() != []
-  requires forall x | x in l.Repr() :: allocated(x)
-  ensures l.Valid()
-  ensures l.Model() == old(l.Model())
-  ensures forall x | x in l.Repr() - old(l.Repr()) :: fresh(x)
-  ensures forall x | x in l.Repr() :: allocated(x)
-{
-  ghost var rep := l.Repr();
-  var it1 := l.Begin();
-
-  ghost var rep2 := l.Repr();
-  var x := it1.Next();
-
-  reprProgression(rep,rep2,l.Repr());
-
-}
-
-/*method IteratorExample2(l: List)
-  modifies l, l.Repr()
-  requires l.Valid()
-  requires l.Model() != []
-  requires forall x | x in l.Repr() :: allocated(x)
-  ensures l.Valid()
-  ensures l.Model() == old(l.Model())
-  ensures forall x | x in l.Repr() - old(l.Repr()) :: fresh(x)
-  ensures forall x | x in l.Repr() :: allocated(x)
-{
-    ghost var rep := l.Repr();
-
-  var it1 := l.Begin();
- assert forall it | it in old(l.Iterators()) && old(it.Valid()) ::
-      it.Valid() && it.Index() == old(it.Index());
-
-     ghost var rep2 := l.Repr();
-          assert forall x | x in l.Repr() - old(l.Repr()) :: fresh(x);
-    assert it1.Valid();
-  assert it1.Index() == 0;
-  assert it1.Index() < |l.Model()|;
-  assert it1.HasNext();
-  assert l.Valid();
-  assert allocated(it1);
-  assert forall x | x in l.Repr()::allocated(x);
-  assert forall it | it in l.Iterators() :: it in l.Repr();
-assert it1 in l.Repr();
-
-  var it2 := l.Begin();
-    assert (l.Repr()-rep) == (l.Repr()-rep2) + (rep2-rep)*l.Repr();
-    assert forall x | x in l.Repr() - rep :: fresh(x);
-
-  assert it2.Valid();
-  assert it2.Index() == 0;
-  assert it2.Index() < |l.Model()|;
-  assert it2.HasNext();
-  assert it1.Valid();
-  assert it1.Index() == 0;
-  assert it1.Index() < |l.Model()|;
-  assert it1.HasNext();
-  var x := it2.Next();
-}*/
-
-/*method IteratorExample3(l: LinkedList)
-  modifies l, l.Repr()
-  requires l.Valid()
-  requires l.Model() != []
-  requires forall x | x in l.Repr() :: allocated(x)
-  ensures l.Valid()
-  ensures forall x | x in l.Repr() - old(l.Repr()) :: fresh(x)
-  ensures forall x | x in l.Repr() :: allocated(x)
-{
-  var it1 := l.Begin();
-  var it2 := l.Begin();
-  var x := it2.Next();
-  var y := l.PopFront();
-  assert x == y;
-  assert !it1.Valid();
-  assert it2.Valid();
-}
-*/
-/*method FindMax(l: LinkedList) returns (max: ListIterator)
-  modifies l, l.Repr()
-  requires l.Valid()
-  requires l.Model() != []
-  requires forall x | x in l.Repr() :: allocated(x)
-  ensures l.Valid()
-  ensures l.Model() == old(l.Model())
-  ensures fresh(max)
-  ensures max.Valid()
-  ensures max.Parent() == l
-  ensures max.HasNext()
-  ensures forall x | x in l.Model() :: l.Model()[max.Index()] >= x
-  ensures forall x | x in l.Repr() - old(l.Repr()) :: fresh(x)
-  ensures forall x | x in l.Repr() :: allocated(x)
-  ensures l.Iterators() >= old(l.Iterators())
-  ensures forall it | it in old(l.Iterators()) && old(it.Valid()) ::
-    it.Valid() && it.Index() == old(it.Index())
-{
-  max := l.Begin();
-  var it := l.Begin();
-  while it.HasNext()
-    decreases |l.Model()| - it.Index()
-    invariant l.Valid()
-    invariant l.Model() == old(l.Model())
-    invariant it.Valid()
-    invariant it.Parent() == l
-    invariant it in l.Iterators()
-    invariant fresh(max)
-    invariant max.Valid()
-    invariant max.Parent() == l
-    invariant max in l.Iterators()
-    invariant max != it
-    invariant max.HasNext()
-    invariant it.Index() <= |l.Model()|
-    invariant forall k | 0 <= k < it.Index() :: l.Model()[max.Index()] >= l.Model()[k]
-    invariant forall x | x in l.Repr() - old(l.Repr()) :: fresh(x)
-    invariant forall x | x in l.Repr() :: allocated(x)
-    invariant forall x | x in old(l.Repr()) :: allocated(x)
-    invariant l.Iterators() >= old(l.Iterators())
-    invariant forall it | it in old(l.Iterators()) && old(it.Valid()) ::
-      it.Valid() && it.Index() == old(it.Index())
-  {
-    if it.Peek() > max.Peek() {
-      max := it.Copy();
-    }
-    var x := it.Next();
-  }
-}*/
-
-function Dup<A>(xs: seq<A>): seq<A>
-{
-  if xs == [] then
-    []
-  else
-    [xs[0]] + [xs[0]] + Dup(xs[1..])
-}
-
-function DupRev<A>(xs: seq<A>): seq<A>
-  ensures 2*|xs| == |DupRev(xs)|
-{
-  if xs == [] then
-    []
-  else
-    DupRev(xs[..|xs|-1]) + [xs[|xs|-1]] + [xs[|xs|-1]]
-}
-
-lemma DupDupRev<A>(xs: seq<A>)
-  ensures Dup(xs) == DupRev(xs)
- {
-   if |xs| <=1 {
-   } else
-    {
-     calc == {
-       Dup(xs);
-       [xs[0]] + [xs[0]] + Dup(xs[1..]);
-       [xs[0]] + [xs[0]] + DupRev(xs[1..]);
-       {assert |xs[1..]|==|xs|-1 >=1;
-       assert xs[1..][|xs|-2]== xs[|xs|-1];
-       assert xs[1..][..|xs|-2]== xs[1..|xs|-1];}
-       [xs[0]] + [xs[0]]  + (DupRev(xs[1..|xs|-1]) + [xs[|xs|-1]] + [xs[|xs|-1]]);
-       DupRev(xs[..|xs|-1]) + [xs[|xs|-1]] + [xs[|xs|-1]];
-       DupRev(xs);
-     }
-   }
- }
-
-method DupElements(l: LinkedList)
-  modifies l, l.Repr()
-  requires l.Valid()
-  requires forall x | x in l.Repr() :: allocated(x)
-  ensures l.Valid()
-  ensures l.Model() == old(Dup(l.Model()))
-  ensures forall x | x in l.Repr() - old(l.Repr()) :: fresh(x)
-  ensures forall x | x in l.Repr() :: allocated(x)
-{
-  ghost var rep := l.Repr();
-
-  var it := l.Begin();
-  ghost var i := 0;
-  while it.HasNext()
-    decreases |l.Model()| - it.Index()
-    invariant l.Valid()
-    invariant 2*i <= |l.Model()|
-    invariant i <= old(|l.Model()|)
-    invariant l.Model()[..2*i] == old(DupRev(l.Model()[..i]))
-    invariant l.Model()[2*i..] == old(l.Model()[i..])
-    invariant it.Parent() == l
-    invariant it.Valid()
-    invariant {it} !! {l}
-    invariant it.Index() == 2*i
-    invariant it in l.Iterators()
-    invariant forall x | x in l.Repr() - old(l.Repr()) :: fresh(x)
-    invariant forall x | x in l.Repr() :: allocated(x)
-  {
-    assert i < old(|l.Model()|);
-    ghost var omodel := l.Model();
-    assert omodel[..2*i] == old(DupRev(l.Model()[..i]));
-
-    ghost var rep2 := l.Repr();
-
-    var x := it.Peek();
-
-    reprProgression(rep,rep2,l.Repr());
-    ghost var rep3 := l.Repr();
-
-    l.Insert(it, x);
-
-    ghost var model := l.Model();
-    calc == {
-      model;
-      Seq.Insert(x, omodel, it.Index());
-      omodel[..it.Index()] + [x] + omodel[it.Index()..];
-      omodel[..2*i+1] + [x] + omodel[2*i+1..];
-      omodel[..2*i] + [x] + [x] + omodel[2*i+1..];
-      old(DupRev(l.Model()[..i])) + [x] + [x] + omodel[2*i+1..];
-      { assert old(l.Model()[i]) == x; }
-      old(DupRev(l.Model()[..i])) + [old(l.Model()[i])] + [old(l.Model()[i])] + omodel[2*i+1..];
-      { assert old(l.Model()[..i+1][..|l.Model()[..i+1]|-1]) == old(l.Model()[..i]); }
-      old(DupRev(l.Model()[..i+1])) + omodel[2*i+1..];
-    }
-    assert model == old(DupRev(l.Model()[..i+1])) + omodel[2*i+1..];
-
-    reprProgression(rep,rep3,l.Repr());
-    ghost var rep4 := l.Repr();
-
-    x := it.Next();
-
-    reprProgression(rep,rep4,l.Repr());
-
-    i := i + 1;
-  }
-
-  calc == {
-    l.Model();
-    l.Model()[..2*i];
-    old(DupRev(l.Model()[..i]));
-    { assert old(l.Model()[..i]) == old(l.Model()); }
-    old(DupRev(l.Model()));
-    { DupDupRev(old(l.Model())); }
-    old(Dup(l.Model()));
-  }
-  assert l.Model() == old(Dup(l.Model()));
+    ensures fresh(next)
+    ensures Iterators() == {next}+old(Iterators())
+    ensures next.Valid() && next.Index()==old(mid.Index())
+    ensures forall it | it in old(Iterators()) && old(it.Valid()) && old(it.Index()) != old(mid.Index()) :: it.Valid()
+    ensures forall it | it in old(Iterators()) && old(it.Valid()) && old(it.Index()) != old(mid.Index()) ::
+      if old(it.Index()) < old(mid.Index())  then
+        it.Index() == old(it.Index())
+      else
+        it.Index() == old(it.Index()) - 1
 }
